src/log_lemmas.lean
@@ -4,6 +4,13 @@ import tactic
 
 namespace nat
 
+lemma lt_pow_succ_log_self' {b : ℕ} (hb : 1 < b) (x : ℕ) : x < b^(log b x + 1) :=
+begin
+  cases x, { simp, linarith, },
+  apply lt_pow_succ_log_self hb,
+  simp,
+end
+
 lemma log_pow_k_le (b x k : ℕ) : log b (x^k) ≤ k * (log b x + 1) :=
 begin
   cases b, { simp, }, cases b, { simp, },
@@ -11,8 +18,7 @@ begin
   suffices : x^k ≤ b'^(k*(log b' x+1)),
   { refine (log_le_log_of_le this).trans _, rw log_pow one_lt, },
   rw pow_mul', mono,
-  cases x, { exact zero_le _, },
-  apply le_of_lt, apply lt_pow_succ_log_self; simp,
+  apply le_of_lt, apply lt_pow_succ_log_self' one_lt,
 end
 
 lemma log_succ_le (b x : ℕ) : log b (x + 1) ≤ x :=
@@ -23,5 +29,10 @@ begin
   apply le_of_lt_succ, simp only [nat.succ_eq_add_one, add_lt_add_iff_right],
   apply lt_pow_self, simp,
 end
+
+lemma lt_pow_succ_of_log_le {b x y : ℕ} (hb : 1 < b) (h : log b x ≤ y) : x < b^(y+1) :=
+calc x < b^(log b x + 1) : lt_pow_succ_log_self' hb x
+   ... ≤ b^(y + 1) : by { apply pow_mono (le_of_lt hb), simpa, }
+
 
 end nat
